Zcash/Circuits/NoteCommit/Composites.lean
@@ -102,11 +102,15 @@ def circuit :
 
   synthesize := fun (gcfg, lcfg) input => synth gcfg lcfg input
 
-  elaborated := fun (gcfg, lcfg) =>
-    { output := fun _ _ => ()
-      regionCount := fun _ => 2
-      output_eq := by intro _ _; rfl
-      regionCount_eq := fun input i => (synth_regionCount gcfg lcfg input i).symm }
+  elaborated :=
+    { keygenRequirements :=
+        { gates cfg _ := [GdCanonicity.gate cfg.1]
+          lookups cfg _ := [LookupRangeCheck.rangeCheckLookup 10 cfg.2] }
+      output _ _ _ := ()
+      regionCount _ := 2
+      output_eq := by intro _ _ _; rfl
+      regionCount_eq := fun (gcfg, lcfg) input i =>
+        (synth_regionCount gcfg lcfg input i).symm }
 
   EnvAssumptions := fun (_, lcfg) env =>
     LookupRangeCheck.TableLoaded 10 lcfg env.env ∧
@@ -250,11 +254,15 @@ def circuit :
 
   synthesize := fun (gcfg, lcfg) input => synth gcfg lcfg input
 
-  elaborated := fun (gcfg, lcfg) =>
-    { output := fun _ _ => ()
-      regionCount := fun _ => 2
-      output_eq := by intro _ _; rfl
-      regionCount_eq := fun input i => (synth_regionCount gcfg lcfg input i).symm }
+  elaborated :=
+    { keygenRequirements :=
+        { gates cfg _ := [PkdCanonicity.gate cfg.1]
+          lookups cfg _ := [LookupRangeCheck.rangeCheckLookup 10 cfg.2] }
+      output _ _ _ := ()
+      regionCount _ := 2
+      output_eq := by intro _ _ _; rfl
+      regionCount_eq := fun (gcfg, lcfg) input i =>
+        (synth_regionCount gcfg lcfg input i).symm }
 
   EnvAssumptions := fun (_, lcfg) env =>
     LookupRangeCheck.TableLoaded 10 lcfg env.env ∧
@@ -391,11 +399,15 @@ def circuit :
 
   synthesize := fun (gcfg, lcfg) input => synth gcfg lcfg input
 
-  elaborated := fun (gcfg, lcfg) =>
-    { output := fun _ _ => ()
-      regionCount := fun _ => 2
-      output_eq := by intro _ _; rfl
-      regionCount_eq := fun input i => (synth_regionCount gcfg lcfg input i).symm }
+  elaborated :=
+    { keygenRequirements :=
+        { gates cfg _ := [RhoCanonicity.gate cfg.1]
+          lookups cfg _ := [LookupRangeCheck.rangeCheckLookup 10 cfg.2] }
+      output _ _ _ := ()
+      regionCount _ := 2
+      output_eq := by intro _ _ _; rfl
+      regionCount_eq := fun (gcfg, lcfg) input i =>
+        (synth_regionCount gcfg lcfg input i).symm }
 
   EnvAssumptions := fun (_, lcfg) env =>
     LookupRangeCheck.TableLoaded 10 lcfg env.env ∧
@@ -533,11 +545,15 @@ def circuit :
 
   synthesize := fun (gcfg, lcfg) input => synth gcfg lcfg input
 
-  elaborated := fun (gcfg, lcfg) =>
-    { output := fun _ _ => ()
-      regionCount := fun _ => 2
-      output_eq := by intro _ _; rfl
-      regionCount_eq := fun input i => (synth_regionCount gcfg lcfg input i).symm }
+  elaborated :=
+    { keygenRequirements :=
+        { gates cfg _ := [PsiCanonicity.gate cfg.1]
+          lookups cfg _ := [LookupRangeCheck.rangeCheckLookup 10 cfg.2] }
+      output _ _ _ := ()
+      regionCount _ := 2
+      output_eq := by intro _ _ _; rfl
+      regionCount_eq := fun (gcfg, lcfg) input i =>
+        (synth_regionCount gcfg lcfg input i).symm }
 
   EnvAssumptions := fun (_, lcfg) env =>
     LookupRangeCheck.TableLoaded 10 lcfg env.env ∧
