Zcash/Circuits/NoteCommit/YComposite.lean
@@ -211,15 +211,22 @@ def circuit (wlsb : WitgenIR Fp 1) :
 
   synthesize := fun (gcfg, lcfg) input => synth wlsb gcfg lcfg input
 
-  elaborated := fun (gcfg, lcfg) =>
-    { output := fun input i => .of (i + 4) 0 (gcfg.advices 6)
-      regionCount := fun _ => 5
+  elaborated :=
+    { keygenRequirements :=
+        { gates cfg _ :=
+            [YCanonicity.gate cfg.1, LookupRangeCheck.bitshiftGate 10 cfg.2]
+          lookups cfg _ := [LookupRangeCheck.rangeCheckLookup 10 cfg.2] }
+      registered _ _ _ _ _ := by
+        keygen_registration
+      output cfg _ i := .of (i + 4) 0 (cfg.1.advices 6)
+      regionCount _ := 5
       output_eq := by
-        intro input i
+        intro (gcfg, lcfg) input i
         simp only [synth, LookupRangeCheck.witnessShortCheck, LookupRangeCheck.witnessCheck,
           LookupRangeCheck.witnessCheckDecomposed, circuit_norm]
         rfl
-      regionCount_eq := fun input i => (synth_regionCount wlsb gcfg lcfg input i).symm }
+      regionCount_eq := fun (gcfg, lcfg) input i =>
+        (synth_regionCount wlsb gcfg lcfg input i).symm }
 
   EnvAssumptions := fun (_, lcfg) env =>
     LookupRangeCheck.TableLoaded 10 lcfg env.env ∧
